Pyramid.fst
@@ -10,7 +10,9 @@ open FStar.UInt
 
 type msg = {
   sender : UInt160.t;
+  this : UInt160.t;
   value: UInt256.t;
+  now : UInt256.t;
 }
 
 val set : #key:eqtype -> #vl:Type -> (key -> vl) -> key -> vl -> (key -> vl)
@@ -24,6 +26,25 @@ let address_to_uint a =
   let x : uint_t 160 = UInt160.v a in
   let y : uint_t 256 = UInt.to_uint_t 256 x in
   UInt256.uint_to_t y
+
+val uint_to_address : UInt256.t -> UInt160.t
+let uint_to_address a = UInt160.uint_to_t (UInt.to_uint_t 160 (UInt256.v a))
+
+val list_length : #a:Type -> list a -> UInt256.t
+let list_length #a lst = UInt256.uint_to_t (UInt.to_uint_t 256 (List.length lst))
+
+val list_nth : #a:Type -> list a -> UInt256.t -> ML a
+let list_nth #a lst n = List.nth lst (UInt256.v n)
+
+val list_set : #a:Type -> list a -> UInt256.t -> a -> ML (list a)
+let list_set #a lst n elem =
+  let n = UInt256.v n in
+  List.mapi (fun i a -> if i = n then elem else a) lst 
+
+val update_balance : UInt160.t -> UInt160.t -> UInt256.t -> (UInt160.t -> UInt256.t) -> (UInt160.t -> UInt256.t)
+let update_balance sender addr v bal x =
+   if addr = x then UInt256.add_mod v (bal x) else
+   if addr = sender then UInt256.sub_mod (bal x) v else bal x
 
 exception SolidityThrow
 exception SolidityReturn
@@ -40,11 +61,13 @@ let bool_and a b = a && b
 val bool_or : bool -> bool -> Tot bool
 let bool_or a b = a || b
 
+type event = unit
 
 
 
 (* Storage state *)
 noeq type state = {
+events__: list event; balance__ : UInt160.t -> UInt256.t;
 parent : UInt160.t -> UInt160.t;
 balance : UInt160.t -> UInt256.t;
 invite : UInt160.t -> UInt160.t;
@@ -65,6 +88,9 @@ let uint256_3 = UInt256.uint_to_t (3)
 
 
 
+assume type inv : state -> Type
+assume val call_env : state -> state
+assume val call_spec : st:state -> Lemma (requires inv st) (ensures inv (call_env st))
 
 
 
@@ -84,12 +110,12 @@ let method_doInvite msg state addr =
 let s = alloc state in
 let ret = alloc None in
 try
-if op_disEquality (get (!s).invite (addr)) (address_0)
+if op_disEquality ((get (!s).invite (addr))) (address_0)
 then (raise SolidityThrow; ())
 else ();
 
 s := {!s with invite = set (!s).invite (addr) ((msg).sender) };
-s := {!s with invites_left = set (!s).invites_left ((msg).sender) (UInt256.sub_mod (get (!s).invites_left ((msg).sender)) (uint256_1)) };
+s := {!s with invites_left = set (!s).invites_left ((msg).sender) (UInt256.sub_mod ((get (!s).invites_left ((msg).sender))) (uint256_1)) };
 (!ret, !s)
 with SolidityReturn -> (!ret, !s)
 
@@ -99,12 +125,12 @@ let method_cancelInvite msg state addr =
 let s = alloc state in
 let ret = alloc None in
 try
-if bool_or (get (!s).joined (addr)) (op_disEquality (get (!s).invite (addr)) ((msg).sender))
+if bool_or ((get (!s).joined (addr))) (op_disEquality ((get (!s).invite (addr))) ((msg).sender))
 then (raise SolidityThrow; ())
 else ();
 
 s := {!s with invite = set (!s).invite (addr) (address_0) };
-s := {!s with invites_left = set (!s).invites_left ((msg).sender) (UInt256.add_mod (get (!s).invites_left ((msg).sender)) (uint256_1)) };
+s := {!s with invites_left = set (!s).invites_left ((msg).sender) (UInt256.add_mod ((get (!s).invites_left ((msg).sender))) (uint256_1)) };
 (!ret, !s)
 with SolidityReturn -> (!ret, !s)
 
@@ -114,10 +140,14 @@ let method_pull msg state () =
 let s = alloc state in
 let ret = alloc None in
 try
-let sum = alloc (get (!s).balance ((msg).sender)) in
+let sum = alloc ((get (!s).balance ((msg).sender))) in
 
 s := {!s with balance = set (!s).balance ((msg).sender) (uint256_0) };
-();
+(let value__ = !sum in
+let recv__ = (msg).sender in
+if UInt256.lt ((!s).balance__ msg.this) value__ then raise SolidityThrow else
+( s := {!s with balance__ = update_balance msg.this recv__ value__ (!s).balance__};
+  s := call_env !s ));
 (!ret, !s)
 with SolidityReturn -> (!ret, !s)
 
@@ -131,12 +161,12 @@ if UInt256.lt ((msg).value) (uint256_1)
 then (raise SolidityThrow; ())
 else ();
 
-if get (!s).joined ((msg).sender)
+if (get (!s).joined ((msg).sender))
 then (raise SolidityThrow; ())
 else ();
 
-if bool_and (op_disEquality (get (!s).invite ((msg).sender)) (address_0)) (UInt256.gt (get (!s).invites_left (get (!s).invite ((msg).sender))) (uint256_0))
-then (let par = alloc (get (!s).invite ((msg).sender)) in
+if bool_and (op_disEquality ((get (!s).invite ((msg).sender))) (address_0)) (UInt256.gt ((get (!s).invites_left ((get (!s).invite ((msg).sender))))) (uint256_0))
+then (let par = alloc ((get (!s).invite ((msg).sender))) in
 
 s := {!s with parent = set (!s).parent ((msg).sender) (!par) };
 s := {!s with joined = set (!s).joined ((msg).sender) (true) };
@@ -144,9 +174,10 @@ s := {!s with invites_left = set (!s).invites_left ((msg).sender) (uint256_3) };
 let i = alloc (uint256_0) in
 let rec loop_199 () : ML unit =
 if not (UInt256.lt (!i) (uint256_10)) then () else (
-s := {!s with balance = set (!s).balance (!par) (UInt256.add_mod (get (!s).balance (!par)) (let (ret,st) = method_calc msg !s
-!i in (s := st; match ret with Some x -> x | None -> (* assert False ; *) raise SolidityBadReturn))) };
-par := get (!s).parent (!par);i := UInt256.add_mod (!i) (uint256_1);loop_199 ()) in loop_199(); ())
+s := {!s with balance = set (!s).balance (!par) (UInt256.add_mod ((get (!s).balance (!par))) ((let (ret__,st__) = method_calc msg !s
+!i in
+ (s := st__; match ret__ with Some x -> x | None -> (* assert False ; *) raise SolidityBadReturn)))) };
+par := (get (!s).parent (!par));i := UInt256.add_mod (!i) (uint256_1);loop_199 ()) in loop_199(); ())
 else ();
 
 (!ret, !s)
