Token.fst
@@ -10,7 +10,9 @@ open FStar.UInt
 
 type msg = {
   sender : UInt160.t;
+  this : UInt160.t;
   value: UInt256.t;
+  now : UInt256.t;
 }
 
 val set : #key:eqtype -> #vl:Type -> (key -> vl) -> key -> vl -> (key -> vl)
@@ -24,6 +26,25 @@ let address_to_uint a =
   let x : uint_t 160 = UInt160.v a in
   let y : uint_t 256 = UInt.to_uint_t 256 x in
   UInt256.uint_to_t y
+
+val uint_to_address : UInt256.t -> UInt160.t
+let uint_to_address a = UInt160.uint_to_t (UInt.to_uint_t 160 (UInt256.v a))
+
+val list_length : #a:Type -> list a -> UInt256.t
+let list_length #a lst = UInt256.uint_to_t (UInt.to_uint_t 256 (List.length lst))
+
+val list_nth : #a:Type -> list a -> UInt256.t -> ML a
+let list_nth #a lst n = List.nth lst (UInt256.v n)
+
+val list_set : #a:Type -> list a -> UInt256.t -> a -> ML (list a)
+let list_set #a lst n elem =
+  let n = UInt256.v n in
+  List.mapi (fun i a -> if i = n then elem else a) lst 
+
+val update_balance : UInt160.t -> UInt160.t -> UInt256.t -> (UInt160.t -> UInt256.t) -> (UInt160.t -> UInt256.t)
+let update_balance sender addr v bal x =
+   if addr = x then UInt256.add_mod v (bal x) else
+   if addr = sender then UInt256.sub_mod (bal x) v else bal x
 
 exception SolidityThrow
 exception SolidityReturn
@@ -40,13 +61,18 @@ let bool_and a b = a && b
 val bool_or : bool -> bool -> Tot bool
 let bool_or a b = a || b
 
+type event = unit
 
 
 
 (* Storage state *)
 noeq type state = {
+events__: list event; balance__ : UInt160.t -> UInt256.t;
 balance : UInt160.t -> UInt256.t;
 }
+assume type inv : state -> Type
+assume val call_env : state -> state
+assume val call_spec : st:state -> Lemma (requires inv st) (ensures inv (call_env st))
 
 
 
@@ -66,11 +92,11 @@ let method_send msg state a amount =
 let s = alloc state in
 let ret = alloc None in
 try
-if UInt256.lt (get (!s).balance ((msg).sender)) (amount)
+if UInt256.lt ((get (!s).balance ((msg).sender))) (amount)
 then (raise SolidityThrow; ())
 else ();
 
-s := {!s with balance = set (!s).balance ((msg).sender) (UInt256.sub_mod (get (!s).balance ((msg).sender)) (amount)) };
-s := {!s with balance = set (!s).balance (a) (UInt256.add_mod (get (!s).balance (a)) (amount)) };
+s := {!s with balance = set (!s).balance ((msg).sender) (UInt256.sub_mod ((get (!s).balance ((msg).sender))) (amount)) };
+s := {!s with balance = set (!s).balance (a) (UInt256.add_mod ((get (!s).balance (a))) (amount)) };
 (!ret, !s)
 with SolidityReturn -> (!ret, !s)
